Rename BlockCache.dfy, merge with master, fix bug in Makefile.template

disk-betree/DiskBetree.dfy
@@ -1,11 +1,11 @@
-include "BlockCache.dfy"  
+include "BlockInterface.dfy"  
 include "../lib/sequences.dfy"
 include "../lib/Maps.dfy"
 include "MapSpec.dfy"
 
 abstract module DiskBetree {
   import MS: MapSpec
-  import BC : BlockCache
+  import BI : BlockInterface
   import opened Sequences
   import opened Maps
   
@@ -14,10 +14,10 @@ abstract module DiskBetree {
   datatype BufferEntry<Value> = Insertion(value: Value)
 
   type Buffer<Value> = imap<Key, seq<BufferEntry<Value>>>
-  //datatype Slot = Slot(child: BC.Reference, buffer: Buffer);
-  datatype Node<Value> = Node(children: imap<Key, BC.Reference>, buffer: Buffer<Value>)
+  //datatype Slot = Slot(child: BI.Reference, buffer: Buffer);
+  datatype Node<Value> = Node(children: imap<Key, BI.Reference>, buffer: Buffer<Value>)
 
-  datatype Layer<Value> = Layer(ref: BC.Reference, node: Node<Value>, accumulatedBuffer: seq<BufferEntry>)
+  datatype Layer<Value> = Layer(ref: BI.Reference, node: Node<Value>, accumulatedBuffer: seq<BufferEntry>)
   type Lookup<Value> = seq<Layer>
 
   predicate BufferIsDefining(log: seq<BufferEntry>) {
@@ -39,7 +39,7 @@ abstract module DiskBetree {
     && (forall i :: 0 <= i < |lookup| - 1 ==> lookup[i].node.children[key] == lookup[i+1].ref)
   }
   
-  predicate LookupRespectsDisk<Value>(view: BC.View<Node<Value>>, lookup: Lookup) {
+  predicate LookupRespectsDisk<Value>(view: BI.View<Node<Value>>, lookup: Lookup) {
     forall i :: 0 <= i < |lookup| ==> IMapsTo(view, lookup[i].ref, lookup[i].node)
   }
 
@@ -54,29 +54,29 @@ abstract module DiskBetree {
     && (forall i :: 0 < i < |lookup| ==> lookup[i].accumulatedBuffer == lookup[i-1].accumulatedBuffer + lookup[i].node.buffer[key])
   }
 
-  predicate IsPathFromRootLookup<Value>(k: Constants, view: BC.View<Node<Value>>, key: Key, lookup: Lookup) {
+  predicate IsPathFromRootLookup<Value>(k: Constants, view: BI.View<Node<Value>>, key: Key, lookup: Lookup) {
     && |lookup| > 0
-    && lookup[0].ref == BC.Root(k.bck)
+    && lookup[0].ref == BI.Root(k.bck)
     && LookupRespectsDisk(view, lookup)
     && LookupFollowsChildRefs(key, lookup)
   }
 
-  predicate IsSatisfyingLookup<Value>(k: Constants, view: BC.View<Node<Value>>, key: Key, value: Value, lookup: Lookup) {
+  predicate IsSatisfyingLookup<Value>(k: Constants, view: BI.View<Node<Value>>, key: Key, value: Value, lookup: Lookup) {
     && IsPathFromRootLookup(k, view, key, lookup)
     && LookupVisitsWFNodes(lookup)
     && LookupAccumulatesMessages(key, lookup)
     && BufferDefinesValue(Last(lookup).accumulatedBuffer, value)
   }
 
-  function Successors(node: Node) : iset<BC.Reference>
+  function Successors(node: Node) : iset<BI.Reference>
   {
     iset k | k in node.children :: node.children[k]
   }
   
   // Now we define the state machine
   
-  datatype Constants = Constants(bck: BC.Constants)
-  datatype Variables<Value> = Variables(bcv: BC.Variables<Node<Value>>)
+  datatype Constants = Constants(bck: BI.Constants)
+  datatype Variables<Value> = Variables(bcv: BI.Variables<Node<Value>>)
 
   function EmptyNode<Value>() : Node {
     var buffer := imap key | MS.InDomain(key) :: [Insertion(MS.EmptyValue())];
@@ -84,13 +84,13 @@ abstract module DiskBetree {
   }
     
   predicate Init(k: Constants, s: Variables) {
-    && BC.Init(k.bck, s.bcv)
-    && IMapsTo(BC.ViewOf(k.bck, s.bcv), BC.Root(k.bck), EmptyNode())
+    && BI.Init(k.bck, s.bcv)
+    && IMapsTo(BI.ViewOf(k.bck, s.bcv), BI.Root(k.bck), EmptyNode())
   }
     
   predicate Query<Value>(k: Constants, s: Variables, s': Variables, key: Key, value: Value, lookup: Lookup) {
     && s == s'
-    && IsSatisfyingLookup(k, BC.ViewOf(k.bck, s.bcv), key, value, lookup)
+    && IsSatisfyingLookup(k, BI.ViewOf(k.bck, s.bcv), key, value, lookup)
   }
 
   function AddMessageToBuffer(buffer: Buffer, key: Key, msg: BufferEntry) : Buffer
@@ -106,16 +106,16 @@ abstract module DiskBetree {
   }
   
   predicate InsertMessage<Value>(k: Constants, s: Variables, s': Variables, key: Key, msg: BufferEntry, oldroot: Node) {
-    && IMapsTo(BC.ViewOf(k.bck, s.bcv), BC.Root(k.bck), oldroot)
+    && IMapsTo(BI.ViewOf(k.bck, s.bcv), BI.Root(k.bck), oldroot)
     && WFNode(oldroot)
     && var newroot := AddMessageToNode(oldroot, key, msg);
-    && BC.Apply(k.bck, s.bcv, s'.bcv, BC.WriteOp(BC.Root(k.bck), newroot, Successors(newroot)))
+    && BI.Apply(k.bck, s.bcv, s'.bcv, BI.WriteOp(BI.Root(k.bck), newroot, Successors(newroot)))
   }
 
-  predicate Flush<Value>(k: Constants, s: Variables, s': Variables, parentref: BC.Reference, parent: Node, childref: BC.Reference, child: Node, newchildref: BC.Reference) {
+  predicate Flush<Value>(k: Constants, s: Variables, s': Variables, parentref: BI.Reference, parent: Node, childref: BI.Reference, child: Node, newchildref: BI.Reference) {
     var movedKeys := iset k | k in parent.children && parent.children[k] == childref;
-    && IMapsTo(BC.ViewOf(k.bck, s.bcv), parentref, parent)
-    && IMapsTo(BC.ViewOf(k.bck, s.bcv), childref, child)
+    && IMapsTo(BI.ViewOf(k.bck, s.bcv), parentref, parent)
+    && IMapsTo(BI.ViewOf(k.bck, s.bcv), childref, child)
     && WFNode(parent)
     && WFNode(child)
     && var newbuffer := imap k :: (if k in movedKeys then parent.buffer[k] + child.buffer[k] else child.buffer[k]);
@@ -123,27 +123,27 @@ abstract module DiskBetree {
     && var newparentbuffer := imap k :: (if k in movedKeys then [] else parent.buffer[k]);
     && var newparentchildren := imap k | k in parent.children :: (if k in movedKeys then newchildref else parent.children[k]);
     && var newparent := Node(newparentchildren, newparentbuffer);
-    && var allocop := BC.AllocOp(newchild, Successors(newchild), newchildref);
-    && var writeop := BC.WriteOp(parentref, newparent, Successors(newparent));
-    && BC.Apply2(k.bck, s.bcv, s'.bcv, allocop, writeop)
+    && var allocop := BI.AllocOp(newchild, Successors(newchild), newchildref);
+    && var writeop := BI.WriteOp(parentref, newparent, Successors(newparent));
+    && BI.Apply2(k.bck, s.bcv, s'.bcv, allocop, writeop)
   }
 
-  predicate Grow(k: Constants, s: Variables, s': Variables, oldroot: Node, newchildref: BC.Reference) {
-    && IMapsTo(BC.ViewOf(k.bck, s.bcv), BC.Root(k.bck), oldroot)
+  predicate Grow(k: Constants, s: Variables, s': Variables, oldroot: Node, newchildref: BI.Reference) {
+    && IMapsTo(BI.ViewOf(k.bck, s.bcv), BI.Root(k.bck), oldroot)
     && var newchild := oldroot;
     && var newroot := Node(
         imap key | MS.InDomain(key) :: newchildref,
         imap key | MS.InDomain(key) :: []);
-    && var allocop := BC.AllocOp(newchild, Successors(newchild), newchildref);
-    && var writeop := BC.WriteOp(BC.Root(k.bck), newroot, Successors(newroot));
-    && BC.Apply2(k.bck, s.bcv, s'.bcv, allocop, writeop)
+    && var allocop := BI.AllocOp(newchild, Successors(newchild), newchildref);
+    && var writeop := BI.WriteOp(BI.Root(k.bck), newroot, Successors(newroot));
+    && BI.Apply2(k.bck, s.bcv, s'.bcv, allocop, writeop)
   }
 
   datatype Step<Value(!new)> =
     | QueryStep(key: Key, value: Value, lookup: Lookup)
     | InsertMessageStep(key: Key, msg: BufferEntry, oldroot: Node)
-    | FlushStep(parentref: BC.Reference, parent: Node, childref: BC.Reference, child: Node, newchildref: BC.Reference)
-    | GrowStep(oldroot: Node, newchildref: BC.Reference)
+    | FlushStep(parentref: BI.Reference, parent: Node, childref: BI.Reference, child: Node, newchildref: BI.Reference)
+    | GrowStep(oldroot: Node, newchildref: BI.Reference)
 
   predicate NextStep(k: Constants, s: Variables, s': Variables, step: Step) {
     match step {
